compiler/backend/proofs/source_to_sourceIcingProofsScript.sml
@@ -3,21 +3,264 @@
 *)
 
 open source_to_sourceIcingTheory fpOptPropsTheory semanticPrimitivesTheory evaluateTheory
-     terminationTheory;
+     terminationTheory fpSemPropsTheory;
 open preamble;
 
 val _ = new_theory "source_to_sourceIcingProofs";
 
-Theorem isFFIstable_swap_ffi:
-  ! e.
-    isFFIstable e ==>
-      ! ffi1 env ffi2 r.
-        evaluate ffi1 env [e] = (ffi2, r) ==>
-        ? fpOpts.
-          ffi2 = ffi1 with fp_opts := fpOpts
+(* TODO: Move *)
+fun impl_subgoal_tac th =
+  let
+    val hyp_to_prove = lhand (concl th)
+  in
+    SUBGOAL_THEN hyp_to_prove (fn thm => assume_tac (MP th thm))
+  end;
+
+val isPureOp_simp =
+  LIST_CONJ (map (fn (t, c) => EVAL (``isPureOp ^t``))
+    (isPureOp_def |> concl |> dest_forall |> snd
+                  |> dest_eq |> snd |> TypeBase.dest_case |> #3));
+
+Theorem isPureOp_same_ffi:
+  ! refs1 (ffi1 ffi2 : 'a ffi_state) op vl refs2 r.
+    isPureOp op /\
+    do_app (refs1, ffi1) op vl = SOME ((refs2,ffi2), r) ==>
+    ! refs (ffi:'a ffi_state).
+      do_app (refs, ffi) op vl = SOME ((refs, ffi), r)
 Proof
-  cheat (* FIXME *)
+  Cases_on `op` \\ rpt gen_tac
+  \\ fs[isPureOp_simp, do_app_def] \\ rpt (TOP_CASE_TAC \\ fs[])
 QED
+
+Theorem do_if_cases:
+  do_if x e1 e2 = SOME e ==> e = e1 \/ e = e2
+Proof
+  fs[do_if_def] \\ TOP_CASE_TAC \\ fs[]
+QED
+
+Theorem isPureExpList_app[simp]:
+  ! es1 es2. isPureExpList (es1 ++ es2) = (isPureExpList es1 /\ isPureExpList es2)
+Proof
+  Induct_on `es1` \\ fs[isPureExp_def]
+  \\ rpt gen_tac
+  \\ EQ_TAC \\ fs[]
+QED
+
+Theorem isPureExpList_reverse[simp]:
+  isPureExpList (REVERSE es) = isPureExpList es
+Proof
+  Induct_on `es` \\ fs[isPureExp_def]
+  \\ rpt gen_tac \\ EQ_TAC \\ simp[]
+QED
+
+local
+  val pmatch_goal =
+    ``\ env refs1 p v vl.
+        ! r.
+        pmatch env refs1 p v vl = r ==>
+        isPurePat p ==>
+        ! refs2. pmatch env refs2 p v vl = r``
+  val pmatch_list_goal =
+    ``\ env refs1 pl v vl.
+        ! r.
+        pmatch_list env refs1 pl v vl = r ==>
+        isPurePatList pl ==>
+        ! refs2. pmatch_list env refs2 pl v vl = r``
+  val indThm = pmatch_ind |> ISPEC pmatch_goal |> SPEC pmatch_list_goal
+in
+Theorem isPurePat_ignores_ref:
+  (! env refs1 p v vl.
+    ^pmatch_goal env refs1 p v vl)
+  /\
+  (! env refs1 pl v vl.
+    ^pmatch_list_goal env refs1 pl v vl)
+Proof
+  match_mp_tac indThm
+  \\ rpt strip_tac
+  \\ fs[isPurePat_def, pmatch_def] \\ rpt (TOP_CASE_TAC \\ fs[]) \\ rpt strip_tac \\ fs[]
+QED
+end
+
+local
+  val eval_goal =
+    ``\ (s1:'ffi state) env expl.
+        ! s2 r.
+          evaluate s1 env expl = (s2, r) ==>
+          isPureExpList expl /\
+          r <> Rerr (Rabort Rtype_error) ==>
+          ! (s:'ffi state).
+            s.fp_rws = s1.fp_rws /\
+            (! x. x <= (s2.fp_choices - s1.fp_choices) ==> s.fp_opts x = s1.fp_opts x) ==>
+            ? fpOpts.
+              evaluate s env expl =
+                (s with <| fp_opts := fpOpts; fp_choices := s.fp_choices + (s2.fp_choices - s1.fp_choices) |>, r)``;
+  val eval_match_goal =
+    ``\ (s1:'ffi state) env v pl err_v.
+        ! s2 r.
+          isPurePatExpList pl /\
+          evaluate_match s1 env v pl err_v = (s2, r) ==>
+          r <> Rerr (Rabort Rtype_error) ==>
+          ! (s:'ffi state).
+            s.fp_rws = s1.fp_rws /\
+            (! x. x <= (s2.fp_choices - s1.fp_choices) ==> s.fp_opts x = s1.fp_opts x) ==>
+              ? fpOpts.
+              evaluate_match s env v pl err_v =
+                (s with <| fp_opts := fpOpts; fp_choices := s.fp_choices + (s2.fp_choices - s1.fp_choices) |>, r)``;
+  val indThm = terminationTheory.evaluate_ind
+    |> ISPEC eval_goal |> SPEC eval_match_goal
+  val isPureExpList_single_thm =
+    SIMP_RULE std_ss [] (EVAL ``isPureExpList [e] = isPureExp e``);
+  val isPureExpList_Cons_thm =
+    SIMP_RULE std_ss [] (EVAL ``isPureExpList (e::es) = (isPureExp e /\ isPureExpList es)``);
+  val resolve_simple =
+    fn thm => mp_tac thm \\ rpt (disch_then (fn dThm => first_assum (mp_then Any mp_tac dThm)));
+  val fp_inv_tac =
+    rpt strip_tac
+    \\ imp_res_tac evaluate_fp_opts_inv \\ rveq
+    \\ rpt (qpat_x_assum `! x. _ x = _ x` (fn thm => fs[GSYM thm]));
+  val trivial =
+    rpt strip_tac \\ rveq \\ fs[]
+    \\ res_tac \\ fs[state_component_equality];
+in
+Theorem isPureExpList_swap_ffi:
+  (! s1 env expl.
+    ^eval_goal s1 env expl) /\
+  (! s1 env v pl err_v.
+    ^eval_match_goal s1 env v pl err_v)
+Proof
+  irule indThm \\ rpt gen_tac \\ rpt conj_tac
+  \\ rpt gen_tac \\ rpt strip_tac \\ fs[]
+  \\ simp[evaluate_def, isPureExp_def]
+  \\ rpt strip_tac
+  \\ fs[isPureExpList_single_thm]
+  \\ TRY (first_x_assum irule \\ fs[Once isPureExp_def] \\ NO_TAC)
+  \\ TRY (fs[state_component_equality] \\ NO_TAC)
+  \\ TRY (qpat_x_assum `_ = (_, _)` mp_tac)
+  >- (
+    ntac 2 (reverse TOP_CASE_TAC \\ fs[]) >- trivial
+    \\ TOP_CASE_TAC \\ fs[]
+    \\ rpt strip_tac
+    \\ last_x_assum (qspec_then `s` resolve_simple)
+    \\ disch_then impl_subgoal_tac
+    >- fp_inv_tac
+    \\ fs[]
+    \\ rename [`do_if (HD r) e2 e3 = SOME eR`]
+    \\ `isPureExp eR` by (imp_res_tac do_if_cases \\ fs[])
+    \\ res_tac \\ fs[]
+    \\ qmatch_goalsub_abbrev_tac `evaluate sNew env [_]`
+    \\ first_x_assum (qspec_then `sNew` resolve_simple)
+    \\ unabbrev_all_tac \\ fs[state_component_equality]
+    \\ disch_then impl_subgoal_tac
+    >- fp_inv_tac
+    \\ first_x_assum impl_subgoal_tac
+    >- fp_inv_tac
+    \\ imp_res_tac evaluate_fp_opts_inv \\ rveq \\ fs[state_component_equality])
+  >- (
+    ntac 2 (reverse TOP_CASE_TAC \\ fs[]) >- trivial
+    \\ ntac 2 (TOP_CASE_TAC \\ fs[])
+    \\ rpt strip_tac \\ rveq \\ fs[isPureExpList_Cons_thm]
+    \\ first_x_assum (qspec_then `s` impl_subgoal_tac)
+    \\ TRY (rpt conj_tac \\ fp_inv_tac \\ NO_TAC)
+    \\ fs[]
+    \\ rpt (first_x_assum (fn ithm => first_x_assum (fn thm => mp_then Any assume_tac thm ithm)))
+    \\ qmatch_goalsub_abbrev_tac `evaluate sNew env _`
+    \\ first_x_assum (qspec_then `sNew` resolve_simple)
+    \\ unabbrev_all_tac
+    \\ disch_then impl_subgoal_tac
+    \\ TRY (rpt conj_tac \\ fp_inv_tac)
+    \\ fs[state_component_equality])
+  >- (
+    ntac 2 (reverse TOP_CASE_TAC \\ fs[]) >- trivial
+    \\ rpt strip_tac \\ rveq \\ fs[isPureExpList_Cons_thm]
+    \\ first_x_assum (qspec_then `s` resolve_simple)
+    \\ disch_then impl_subgoal_tac
+    >- (rpt conj_tac \\ fp_inv_tac)
+    \\ fs[]
+    \\ qmatch_goalsub_abbrev_tac `evaluate_match sNew env _ _ _`
+    \\ first_x_assum impl_subgoal_tac >- fs[]
+    \\ first_x_assum (qspec_then `sNew` resolve_simple)
+    \\ unabbrev_all_tac
+    \\ disch_then impl_subgoal_tac
+    \\ TRY (rpt conj_tac \\ fp_inv_tac)
+    \\ fs[state_component_equality]
+    \\ fp_inv_tac)
+  >- (
+    ntac 2 (reverse TOP_CASE_TAC \\ fs[])
+    >- (rpt strip_tac \\ rveq \\ fs[]
+        \\ first_x_assum drule
+        \\ disch_then (qspec_then `s with fp_canOpt := T` assume_tac)
+        \\ fs[state_component_equality]
+        \\ res_tac  \\ fs[state_component_equality])
+    \\ rpt strip_tac \\ rveq \\ fs[isPureExpList_Cons_thm]
+    \\ res_tac
+    \\ last_x_assum (qspec_then `s with fp_canOpt := T` assume_tac)
+    \\ fs[state_component_equality]
+    \\ res_tac \\ fs[state_component_equality])
+  >- (TOP_CASE_TAC \\ trivial)
+  >- (
+    ntac 2 (reverse TOP_CASE_TAC \\ fs[]) >- trivial
+    \\ ntac 2 (TOP_CASE_TAC \\ fs[])
+    \\ rpt strip_tac \\ rveq \\ fs[]
+    \\ first_x_assum drule
+    \\ disch_then impl_subgoal_tac
+    \\ TRY (fp_inv_tac \\ NO_TAC)
+    \\ fs[state_component_equality]
+    \\ rename [`do_log lop (HD v) e2 = SOME (Exp eR)`]
+    \\ `eR = e2`
+        by (qpat_x_assum `do_log _ _ _ = SOME (Exp eR)` mp_tac
+            \\ fs[do_log_def]
+            \\ rpt (TOP_CASE_TAC \\ fs[]))
+    \\ rveq
+    \\ first_x_assum drule \\ disch_then assume_tac
+    \\ qmatch_goalsub_abbrev_tac `evaluate sNew env _ = _`
+    \\ first_x_assum (qspec_then `sNew` impl_subgoal_tac)
+    \\ unabbrev_all_tac
+    >- (fs[] \\ fp_inv_tac)
+    \\ fs[state_component_equality]
+    \\ fp_inv_tac)
+  >- (
+    ntac 2 (reverse TOP_CASE_TAC \\ fs[]) >- trivial
+    \\ TOP_CASE_TAC \\ fs[]
+    >- (rveq \\ fs[isPureOp_def])
+    \\ ntac 3 (reverse TOP_CASE_TAC \\ fs[])
+    \\ imp_res_tac isPureOp_same_ffi \\ rveq
+    \\ first_x_assum (qspec_then `s` assume_tac)
+    \\ TOP_CASE_TAC \\ rpt strip_tac \\ rveq \\ fs[shift_fp_opts_def]
+    \\ first_x_assum impl_subgoal_tac
+    \\ TRY (fp_inv_tac)
+    \\ imp_res_tac evaluate_fp_opts_inv
+    \\ fs[shift_fp_opts_def, state_component_equality]
+    \\ rpt (qpat_x_assum `! x. _ x = _ x` ( fn thm => fs[GSYM thm])))
+  >- (
+    TOP_CASE_TAC \\ fs[]
+    \\ ntac 2 (reverse TOP_CASE_TAC \\ fs[]) >- trivial
+    \\ TOP_CASE_TAC \\ fs[]
+    \\ rpt strip_tac \\ rveq
+    \\ first_x_assum drule \\ disch_then impl_subgoal_tac
+    >- fp_inv_tac
+    \\ fs[state_component_equality])
+  >- (
+    ntac 2 (reverse TOP_CASE_TAC \\ fs[]) >- trivial
+    \\ rpt strip_tac \\ fs[]
+    \\ first_x_assum (qspec_then `s` impl_subgoal_tac)
+    >- fp_inv_tac
+    \\ fs[]
+    \\ qmatch_goalsub_abbrev_tac `evaluate sNew _ _ = _`
+    \\ first_x_assum impl_subgoal_tac \\ fs[]
+    \\ first_x_assum (qspec_then `sNew` impl_subgoal_tac)
+    \\ unabbrev_all_tac
+    >- fp_inv_tac
+    \\ fs[state_component_equality]
+    \\ fp_inv_tac)
+  >- (
+    ntac 2 (TOP_CASE_TAC \\ fs[])
+    \\ rpt strip_tac \\ fs[]
+    \\ imp_res_tac (hd (CONJ_LIST 2 (EVAL_RULE isPurePat_ignores_ref)))
+    \\ fs[]
+    \\ res_tac \\ fs[state_component_equality]
+    \\ fp_inv_tac)
+QED
+end
 
 Theorem no_match_word_cond:
   ! w e s1 s2.
@@ -162,6 +405,7 @@ Theorem fp_add_comm_cases:
   ! e.
     (? e1 e2.
       e = (App (FP_bop FP_Add) [e1; e2]) /\
+      isPureExp e /\
       rewriteFPexp [fp_add_comm] (App (FP_bop FP_Add) [e1; e2]) =
         App (FP_bop FP_Add) [e2; e1]) \/
     (rewriteFPexp [fp_add_comm] e = e)
@@ -190,12 +434,10 @@ local
   val eval_fp_opt_inv =
     SIMP_RULE std_ss [] fpSemPropsTheory.evaluate_fp_opts_inv
     |> CONJ_LIST 2 |> hd;
-  fun impl_subgoal_tac th =
-    let
-      val hyp_to_prove = lhand (concl th)
-    in
-      SUBGOAL_THEN hyp_to_prove (fn thm => assume_tac (MP th thm))
-    end;
+  val isPureExp_ignores_state =
+    EVAL_RULE isPureExpList_swap_ffi
+    |> CONJ_LIST 2
+    |> hd
 in
 Theorem fp_add_comm_correct:
   ! (ffi1 ffi2:'ffi state) env e res.
@@ -207,39 +449,105 @@ Theorem fp_add_comm_correct:
         (ffi2 with <| fp_rws := ffi2.fp_rws ++ [fp_add_comm] |>, Rval res)
 Proof
   rpt strip_tac
-  \\ qspec_then `e` assume_tac fp_add_comm_cases
+  \\ qspec_then `e` assume_tac (ONCE_REWRITE_RULE [DISJ_COMM] fp_add_comm_cases)
   \\ fs[]
   >- (
-    fs[evaluate_def] \\ rveq
-    \\ qpat_x_assum `_ = (_, _)` mp_tac
-    \\ rename [`evaluate ffi1 env [e1]`]
-    \\ Cases_on `evaluate ffi1 env [e1]` \\ fs[]
-    \\ rename [`evaluate ffi1 env [e1] = (ffi2, r)`] \\ Cases_on `r` \\ fs[]
-    \\ rename [`evaluate ffi2 env [e2]`]
-    \\ Cases_on `evaluate ffi2 env [e2]` \\ fs[]
-    \\ rename [`evaluate ffi2 env [e2] = (ffi3, r)`] \\ Cases_on `r` \\ fs[]
-    \\ ntac 3 (TOP_CASE_TAC \\ fs[])
-    \\ fs[astTheory.isFpOp_def, astTheory.isFpBool_def]
-    \\ rpt strip_tac \\ rveq
-    \\ fs[shift_fp_opts_def]
-    \\ `isFFIstable e1 /\ isFFIstable e2` by (cheat)
-    \\ `? fpOpts. ffi2 = ffi1 with fp_opts := fpOpts`
-      by (imp_res_tac isFFIstable_swap_ffi)
-    \\ imp_res_tac eval_fp_opt_inv
-    \\ imp_res_tac fp_rws_append_comm
-    \\ qexists_tac
-        `\x.
-          if (x = (ffi3.fp_choices - ffi1.fp_choices) + 1)
-          then [RewriteApp Here (LENGTH ffi1.fp_rws)] ++ ffi1.fp_opts x
-          else ffi1.fp_opts x`
-    \\ qmatch_goalsub_abbrev_tac `evaluate ffi1upd env [e2]`
-    \\ qpat_x_assum `evaluate ffi1 _ _ = _` kall_tac
-    \\ qpat_x_assum `evaluate ffi2 _ _ = _` kall_tac
-    \\ last_x_assum (mp_then Any assume_tac fpSemPropsTheory.evaluate_fp_opt_add_bind_preserving)
-    \\ first_x_assum (qspecl_then [`(ffi3.fp_choices - ffi1.fp_choices) +1`, `ffi1upd.fp_opts`] impl_subgoal_tac)
-    >- (rpt conj_tac \\ fs[state_component_equality]
-        \\ rpt strip_tac \\ unabbrev_all_tac
-        \\ qpat_x_assum `! x. _ = ffi2.fp_opts _` (fn thm => fs[GSYM thm])
+    qexists_tac `ffi1.fp_opts` \\ fs[state_component_equality]
+    \\ imp_res_tac fp_rws_append_comm)
+  \\ fs[evaluate_def] \\ rveq
+  \\ qpat_x_assum `_ = (_, _)` mp_tac
+  \\ rename [`evaluate ffi1 env [e1]`]
+  \\ Cases_on `evaluate ffi1 env [e1]` \\ fs[]
+  \\ rename [`evaluate ffi1 env [e1] = (ffi2, r)`] \\ Cases_on `r` \\ fs[]
+  \\ rename [`evaluate ffi2 env [e2]`]
+  \\ Cases_on `evaluate ffi2 env [e2]` \\ fs[]
+  \\ rename [`evaluate ffi2 env [e2] = (ffi3, r)`] \\ Cases_on `r` \\ fs[]
+  \\ ntac 3 (TOP_CASE_TAC \\ fs[])
+  \\ fs[astTheory.isFpOp_def, astTheory.isFpBool_def]
+  \\ rpt strip_tac \\ rveq
+  \\ ntac 2 (first_x_assum
+      (fn thm => mp_then Any assume_tac isPureExp_ignores_state thm \\ mp_tac thm))
+  \\ rpt strip_tac
+  \\ fs[shift_fp_opts_def, isPureExp_def]
+  \\ rpt (qpat_x_assum `isPureExp _` (fn thm => first_x_assum (fn ithm => mp_then Any assume_tac ithm thm) \\ mp_tac thm))
+  \\ first_x_assum (qspec_then `ffi2 with fp_opts := ffi1.fp_opts` assume_tac)
+  \\ first_x_assum (qspec_then `ffi1 with fp_opts := ffi2.fp_opts` assume_tac)
+  \\ first_x_assum impl_subgoal_tac
+  >- (unabbrev_all_tac
+      \\ imp_res_tac evaluate_fp_opts_inv \\ fs[] \\ rveq \\ fs[])
+  \\ first_x_assum impl_subgoal_tac
+  >- (unabbrev_all_tac
+      \\ imp_res_tac evaluate_fp_opts_inv \\ fs[] \\ rveq \\ fs[])
+  \\ fs[]
+  (* changing state once more for each execution *)
+  \\ ntac 2 (first_x_assum
+      (fn thm => mp_then Any assume_tac isPureExp_ignores_state thm \\ mp_tac thm))
+  \\ rpt strip_tac
+  \\ fs[shift_fp_opts_def, isPureExp_def]
+  \\ rpt (qpat_x_assum `isPureExp _` (fn thm => first_x_assum (fn ithm => mp_then Any assume_tac ithm thm)))
+  \\ qexists_tac
+      `\x.
+        if (x = (ffi3.fp_choices - ffi1.fp_choices) + 1)
+        then [RewriteApp Here (LENGTH ffi1.fp_rws)] ++ ffi1.fp_opts x
+        else
+        if (x <= ffi3.fp_choices - ffi2.fp_choices)
+        then ffi2.fp_opts x
+        else ffi1.fp_opts x`
+  \\ qmatch_goalsub_abbrev_tac `evaluate (ffi1 with <| fp_rws := fp_rws_comm; fp_opts := fp_opts_comm |>) env [e2]`
+  \\ last_x_assum (qspec_then `ffi1 with <| fp_opts := fp_opts_comm |>` impl_subgoal_tac)
+  >- (unabbrev_all_tac
+      \\ imp_res_tac evaluate_fp_opts_inv \\ fs[] \\ rveq \\ fs[])
+  \\ fs[]
+  \\ first_x_assum (mp_then Any assume_tac (hd (CONJ_LIST 2 fp_rws_append_comm)))
+  \\ unabbrev_all_tac
+  \\ fs[state_component_equality]
+
+  \\ last_x_assum (qspec_then `ffi1 with fp_opts := fp_opts_comm` impl_subgoal_tac)
+  >- (fs[] \\ unabbrev_all_tac
+      \\ imp_res_tac evaluate_fp_opts_inv \\ rveq \\ rpt conj_tac \\ fs[])
+      \\ rpt strip_tac
+      \\ rpt (qpat_x_assum `! x. _ x = _ x` (fn thm => fs[GSYM thm]))
+      \\ imp_res_tac fp_
+
+
+
+
+
+
+
+
+
+
+
+
+
+
+
+
+
+
+
+
+
+
+
+
+  \\ `? fpOpts. ffi2 = ffi1 with fp_opts := fpOpts`
+    by (imp_res_tac isFFIstable_swap_ffi \\ fs[state_component_equality])
+  \\ `? fpOpts. ffi3 = ffi1 with fp_opts := fpOpts`
+    by (imp_res_tac isFFIstable_swap_ffi \\ fs[state_component_equality])
+  \\ rveq
+
+  \\ imp_res_tac eval_fp_opt_inv
+  \\ imp_res_tac fp_rws_append_comm
+
+  \\ qpat_x_assum `evaluate ffi1 _ _ = _` kall_tac
+  \\ qpat_x_assum `evaluate ffi2 _ _ = _` kall_tac
+  \\ last_x_assum (mp_then Any assume_tac fpSemPropsTheory.evaluate_fp_opt_add_bind_preserving)
+  \\ first_x_assum (qspecl_then [`(ffi3.fp_choices - ffi1.fp_choices) +1`, `ffi1upd.fp_opts`] impl_subgoal_tac)
+  >- (rpt conj_tac \\ fs[state_component_equality]
+      \\ rpt strip_tac \\ unabbrev_all_tac
+      \\ qpat_x_assum `! x. _ = ffi2.fp_opts _` (fn thm => fs[GSYM thm])
  \\ fs[state_component_equality])
     \\ unabbrev_all_tac
     \\ fs[state_component_equality]
